Weidenbach_Book/IsaSAT/IsaSAT_Restart.thy
@@ -1659,7 +1659,6 @@ proof -
     done
 qed
 
-
 lemma heuristic_rel_incr_restartI[intro!]:
   \<open>heuristic_rel \<A> heur \<Longrightarrow> heuristic_rel \<A> (incr_restart_phase_end heur)\<close>
   by (auto simp: heuristic_rel_def heuristic_rel_stats_def incr_restart_phase_end_def)
